theories/cancellation/ElimRel.v
@@ -529,17 +529,18 @@ Proof using.
 Local Tactic Notation "estep" integer(n) := do n (gstep; econs; i).
 Local Ltac edone := eauto 6 with paco.
 
-Lemma elim_rel_cancel (md: SMod.t) (sp: specmap) T msk N stid (itr: itree _ T)
+Lemma elim_rel_cancel (md: SMod.t) (sp: specmap) T msk sN tN stid ttid (itr: itree _ T)
   (WF: SMod.cancellable md)
   (IMG: img_msk msk)
+  (CALL: call_msk msk)
   :
-  @elim_rel (SMod.sp_from_conc md) T ε
+  @elim_rel (SMod.conc_sp_from md) T ε
     (inline_body (sandboxed_prog (SMod.to_mod ∅ (SMod.cancel md))) 
-      (SB.sandbox msk (SModTr.trans ∅ N stid itr)))
-    (inline_body (sandboxed_prog (SMod.to_mod (SMod.sp_from_conc md) md)) 
-      (SB.sandbox msk (SModTr.trans (SMod.sp_from_conc md) N stid itr))).
+      (SB.sandbox msk (SModTr.trans ∅ sN stid itr)))
+    (inline_body (sandboxed_prog (SMod.to_mod (SMod.conc_sp_from md) md)) 
+      (SB.sandbox msk (SModTr.trans (SMod.conc_sp_from md) tN ttid itr))).
 Proof using.
-  ginit. revert IMG. revert T itr N stid msk. gcofix CIH. i.
+  ginit. revert IMG CALL. revert T itr sN tN stid ttid msk. gcofix CIH. i.
   dup WF. red in WF. dup IMG. red in IMG. des.
   assert (CASE:= case_itrH itr). des; subst.
   - rewrite !SRed.ret !SBRed.ret !MIRed.ret. estep 1.
@@ -558,7 +559,7 @@ Proof using.
       { rewrite SBRed.vis E vis_trigger // MIRed.core. ired. estep 1. }
       destruct ((SMod.fnsems md) !! (Some fn)) eqn: E0; cycle 1.
       { rewrite SBRed.vis E vis_trigger -(bind_ret_r (trigger _)).
-        rewrite {4}/SMod.sp_from_conc. rewrite lookup_insert_ne //. rewrite (lookup_sp_from _ _ None) //.
+        rewrite {4}/SMod.conc_sp_from. rewrite lookup_insert_ne //. rewrite (lookup_sp_from _ _ None) //.
         ired. rewrite SBRed.vis E vis_trigger !MIRed.bind. ired.
         rewrite -(bind_ret_r (trigger _)) !MIRed.call. ired.
         estep 1. rewrite !MIRed.bind. rewrite !lookup_omap /= !lookup_fmap E0 /=. ired.
@@ -566,7 +567,7 @@ Proof using.
         estep 1. }
       destruct o; cycle 1.
       { rewrite SBRed.vis E vis_trigger -(bind_ret_r (trigger _)).
-        rewrite {4}/SMod.sp_from_conc. rewrite lookup_insert_ne //. rewrite (lookup_sp_from _ _ (Some None)) //.
+        rewrite {4}/SMod.conc_sp_from. rewrite lookup_insert_ne //. rewrite (lookup_sp_from _ _ (Some None)) //.
         ired. rewrite SBRed.vis E vis_trigger !MIRed.bind. ired.
         rewrite -(bind_ret_r (trigger _)) !MIRed.call. ired.
         estep 1. rewrite !MIRed.bind. rewrite !lookup_omap /= !lookup_fmap E0 /=. ired.
@@ -575,36 +576,46 @@ Proof using.
       destruct p as [img0 [fsp0 bd0]].
       destruct fsp0; [destruct f|]; cycle 1.
       { rewrite SBRed.vis E vis_trigger -(bind_ret_r (trigger _)).
-        rewrite {4}/SMod.sp_from_conc. rewrite lookup_insert_ne //. rewrite (lookup_sp_from _ _ (Some (Some (img0, (None, bd0))))) //.
+        rewrite {4}/SMod.conc_sp_from. rewrite lookup_insert_ne //. rewrite (lookup_sp_from _ _ (Some (Some (img0, (None, bd0))))) //.
         ired. rewrite SBRed.vis E vis_trigger !MIRed.bind. ired.
         rewrite -(bind_ret_r (trigger _)) !MIRed.call. ired.
         estep 1. rewrite !MIRed.bind. rewrite !lookup_omap /= !lookup_fmap E0 /=. ired.
         rewrite !MIRed.ret. ired. guclo elim_rel_bindC_spec. econs.
         { rewrite /SB.sandbox_body /= /SModTr.trans_fnsem /SModTr.HoareFun.
-          rewrite !SBRed.tau !MIRed.tau. estep 2. ss. gbase. eapply CIH.
-          r in WF0. hexploit WF0; eauto. i; des; eauto. }
+          rewrite !SBRed.tau !MIRed.tau. estep 2. ss. gbase. eapply CIH; eauto.
+          { r in WF0. hexploit WF0; eauto. i; des; eauto. }
+          { r in WF0. hexploit WF0; eauto. i; des; eauto. }
+        }
         i. rewrite !MIRed.tau. ired. estep 2. rewrite !MIRed.ret !bind_ret_l.
         rewrite !SBRed.ret !MIRed.ret !bind_ret_l. gbase. eapply CIH; eauto. }
 
       set (fsp := fspec_mk _ _) in E0.
       rewrite SBRed.vis E vis_trigger -(bind_ret_r (trigger _)).
-      rewrite {4}/SMod.sp_from_conc. rewrite lookup_insert_ne //. rewrite (lookup_sp_from _ _ (Some (Some (img0, (Some fsp, bd0))))) //.
+      rewrite {4}/SMod.conc_sp_from. rewrite lookup_insert_ne //. rewrite (lookup_sp_from _ _ (Some (Some (img0, (Some fsp, bd0))))) //.
       
-      des. erewrite MIRed_HoareCall; et; cycle 1.
-      { rewrite /sp_from /to_sp alist_find_map_snd E0 //. }
-      rewrite SBRed.call E -(bind_ret_r (trigger _)) MIRed.call.
-      rewrite {2}/sandboxed_prog. s. rewrite !alist_find_map_snd E0. s. ired.
-      rewrite /SB.sandbox_body /SModTr.trans_body. s.
-      rewrite SBRed.tau bind_tau MIRed.tau ?bind_tau MIRed.bind. ired.
-      
-      gstep. eapply elim_rel_precond; eauto. i.
-      exists x. split; eauto.
+      erewrite MIRed_HoareCall; et; cycle 1.
+      { rewrite /SMod.conc_sp_from. rewrite lookup_insert_ne //.
+        rewrite (lookup_sp_from _ _ (Some (Some (img0, (Some fsp, bd0))))) //. }
 
-      ired. guclo elim_rel_bindC_spec. econs; [edone|].
+      rewrite MIRed.bind MIRed.call MIRed.bind.
+      rewrite {2}/sandboxed_prog. s. 
+      rewrite lookup_omap !lookup_fmap E0 /= MIRed.bind MIRed.ret bind_ret_l.
+      rewrite /SB.sandbox_body /SModTr.trans_fnsem /= SBRed.tau MIRed.tau. ired.
+
+      gstep. eapply elim_rel_precond; eauto. i.
+      exists x, tN, ttid. split; eauto.
+
+      ired. guclo elim_rel_bindC_spec. econs.
+      { gbase. eapply CIH; eauto.
+        { r in WF0. hexploit WF0; eauto. i; des; eauto. }
+        { r in WF0. hexploit WF0; eauto. i; des; eauto. }
+      }
 
       i. ired. rewrite !MIRed.tau MIRed.ret. ired.
+      rewrite SBRed.ret MIRed.ret bind_ret_l.
       gstep. eapply elim_rel_postcond; et.
-      split; eauto. edone.
+      split; eauto.
+      gbase. eapply CIH; eauto.
     }
     
     (* spawn case *)
